denning-sacco/DS.Messages.fsti
@@ -8,6 +8,26 @@ open CryptoLib
 module LC = LabeledCryptoAPI
 
 
+(* Events required to proof security properties *)
+
+let event_initiate (a b srv:principal) =
+  ("initiate",[string_to_bytes a;string_to_bytes b;string_to_bytes srv])
+let event_certify (a b srv:principal) (pk_a pk_b:bytes) (t:timestamp) (clock_cnt:nat) =
+  ("certify",[string_to_bytes a;string_to_bytes b;string_to_bytes srv;pk_a;pk_b;nat_to_bytes 0 t;nat_to_bytes 0 clock_cnt])
+let event_send_key (a b srv:principal) (pk_a pk_b ck:bytes) (t:timestamp) (clock_cnt:nat) =
+  ("send_key",[string_to_bytes a;string_to_bytes b;string_to_bytes srv;pk_a;pk_b;ck;nat_to_bytes 0 t;nat_to_bytes 0 clock_cnt])
+let event_accept_key (a b srv:principal) (pk_a pk_b ck:bytes) (t:timestamp) (clock_cnt:nat) =
+  ("accept_key",[string_to_bytes a;string_to_bytes b;string_to_bytes srv;pk_a;pk_b;ck;nat_to_bytes 0 t;nat_to_bytes 0 clock_cnt])
+
+
+/// Format of encrypted/signed message parts
+noeq type encsigval =
+  | SigCertP: p:principal -> pk_p:bytes -> t:timestamp -> encsigval
+  | EncSigCommKey: ck:bytes -> t:timestamp -> encsigval
+
+val parse_encsigval_: sesv:bytes -> result encsigval
+
+
 let ds_key_usages : LC.key_usages = LC.default_key_usages
 
 let can_pke_encrypt (i:nat) s pk m = True
@@ -31,11 +51,6 @@ let msg i l = LC.msg ds_global_usage i l
 let is_msg i b l = LC.is_msg ds_global_usage i b l
 
 
-/// Format of encrypted/signed message parts
-noeq type encsigval =
-  | SigCertP: p:principal -> pk_p:bytes -> t:timestamp -> encsigval
-  | EncSigCommKey: ck:bytes -> t:timestamp -> encsigval
-
 let valid_encsigval (i:nat) (esv:encsigval) (l:label) =
   match esv with
   | SigCertP p pk_p t -> is_msg i pk_p l
@@ -49,10 +64,15 @@ val parse_encsigval: #i:nat -> #l:label -> sesv:(msg i l) -> r:(result encsigval
     | _ -> True
   }
 
+val parse_encsigval_lemma: #i:nat -> #l:label -> sesv:(msg i l) ->
+  Lemma (parse_encsigval sesv == parse_encsigval_ sesv)
+
 val parse_serialize_encsigval_lemma: i:nat -> esv:encsigval -> l:label ->
   Lemma (requires (valid_encsigval i esv l))
-        (ensures (parse_encsigval (serialize_encsigval i esv l) == Success esv))
-        [SMTPat (parse_encsigval (serialize_encsigval i esv l))]
+        (ensures (parse_encsigval (serialize_encsigval i esv l) == Success esv /\
+                  parse_encsigval_ (serialize_encsigval i esv l) == Success esv))
+        [SMTPat (parse_encsigval (serialize_encsigval i esv l));
+         SMTPat (parse_encsigval_ (serialize_encsigval i esv l))]
 
 
 noeq type message (i:nat) =
